More progress in defining probabilistic predicates. Improve the definition of global_state.

examples/rnd_hoare/probabilistic_pred.v
@@ -48,98 +48,64 @@ Section Predicates.
 
 Context {imp: Imperative} {sss: SmallStepSemantics} {rhd: RandomHistoryDistribution ora} {drhd: DiscreteRandomHistoryDistribution ora}.
 
-Definition tm_meta_pred (P: state -> Prop): MetaState state -> Prop :=
-  fun s => match s with Terminating s' => P s' | _ => False end.
-
-Definition valid_set (P: MetaState state -> Prop) (sigma: global_state): Ensemble RandomHistory :=
-  fun h => match sigma h with Some s => P s | _ => False end.
-
-Definition ntm_set (sigma: global_state): Ensemble RandomHistory :=
-  valid_set (eq (NonTerminating _)) sigma.
-
-Definition tm_set (P: state -> Prop) (sigma: global_state): Ensemble RandomHistory :=
-  valid_set (tm_meta_pred P) sigma.
-
-Lemma valid_set_measurable: forall (P: MetaState state -> Prop) (sigma: global_state),
-  is_measurable_subspace (DomainOfVar sigma) ->
-  is_measurable_subspace (valid_set P sigma).
-sss 
-(* Not correct. P should be inhabited. *)
+Lemma state_pred_domain_measurable: forall (P: MetaState state -> Prop) (sigma: global_state)
+  (H: is_measurable_subspace (rv_domain _ sigma)),
+  is_measurable_set (exist _ _ H) (element_pred_domain P sigma).
 Admitted.
-
-Lemma valid_set_Dom: forall (P: MetaState state -> Prop) (sigma: global_state),
-  Included _ (valid_set P sigma) (DomainOfVar sigma).
-Proof.
-  unfold Included, Ensembles.In; intros.
-  unfold valid_set in H.
-  change ((DomainOfVar sigma) x) with (isSome (sigma x)).
-  destruct (sigma x); simpl; auto.
-Qed.
 
 (***************************)
 (* overload global state   *)
 (***************************)
 
-Definition global_state: Type := {sigma: global_state | is_measurable_subspace (DomainOfVar sigma)}.
+Definition global_state: Type := {sigma: global_state | is_measurable_subspace (rv_domain _ sigma)}.
 
 Definition global_state_MSS (sigma: global_state): {P: RandomHistory -> Prop | is_measurable_subspace P} :=
-  exist is_measurable_subspace (DomainOfVar (proj1_sig sigma)) (proj2_sig sigma).
+  exist is_measurable_subspace (rv_domain _ (proj1_sig sigma)) (proj2_sig sigma).
 
-Definition valid_set_MSS (P: MetaState state -> Prop) (sigma: global_state): {P: RandomHistory -> Prop | is_measurable_subspace P}.
-  exists (valid_set P (proj1_sig sigma)).
-  apply valid_set_measurable, (proj2_sig sigma).
-Defined.
-
-Definition valid_set_MS (P: MetaState state -> Prop) (sigma: global_state): measurable_set (global_state_MSS sigma).
-  exists (valid_set P (proj1_sig sigma)).
+Definition state_pred_domain_MS (P: MetaState state -> Prop) (sigma: global_state): measurable_set (global_state_MSS sigma).
+  exists (element_pred_domain P (proj1_sig sigma)).
   split.
-  + apply valid_set_Dom.
-  + apply (measurable_subset_measurable (global_state_MSS sigma) (valid_set_MSS P sigma)).
-    apply valid_set_Dom.
+  + exact (element_pred_domain_Dom _ _).
+  + apply (state_pred_domain_measurable P (proj1_sig sigma)).
 Defined.
 
-Definition ntm_set_MS (sigma: global_state): measurable_set (global_state_MSS sigma) :=
-  valid_set_MS (eq (NonTerminating _)) sigma.
+Definition ntm_pred_MS (sigma: global_state): measurable_set (global_state_MSS sigma) :=
+  state_pred_domain_MS (eq (NonTerminating _)) sigma.
 
-Definition tm_set_MS (P: state -> Prop) (sigma: global_state): measurable_set (global_state_MSS sigma) :=
-  valid_set_MS (tm_meta_pred P) sigma.
+Definition tm_pred_MS (P: state -> Prop) (sigma: global_state): measurable_set (global_state_MSS sigma) :=
+  state_pred_domain_MS (tm_meta_pred P) sigma.
 
-Definition Pr (P: state -> Prop) (sigma: global_state): R := GProb (ms_construct _ _ (proj2_sig sigma)).
+Definition Pr (P: state -> Prop) (sigma: global_state): R := measure_of _ (tm_pred_MS P sigma).
 
-Definition nPr {imp: Imperative} {sss: SmallStepSemantics} {psi: RandomDistribution ora} (sigma: global_state): R := GProb (ntm_set sigma).
+Definition nPr (sigma: global_state): R := measure_of _ (ntm_pred_MS sigma).
 
-Definition PTriple {imp: Imperative} {sss: SmallStepSemantics} {psi: RandomDistribution ora} (P: global_state -> Prop) (c: cmd) (Q: global_state -> Prop): Prop :=
-  forall p (s1: global_state),
+Definition RCPPred (P: global_state -> Prop) (filter: state -> Prop) (sigma: global_state): Prop :=
+  ~ is_measurable_subspace (tm_domain filter (proj1_sig sigma)) /\
+  exists M: is_measurable_subspace (tm_domain filter (proj1_sig sigma)),
+  P (exist _ (element_pred_filter_global_state (tm_meta_pred filter) (proj1_sig sigma)) M).
+
+Definition ExPred {A: Type} (P: A -> global_state -> Prop) (sigma: global_state): Prop := exists a: A, P a sigma.
+
+Definition ExrPred {A: Type} (P: A -> global_state -> Prop) (sigma: global_state): Prop := exists a: A, P a sigma.
+
+
+Definition PTriple (P: global_state -> Prop) (c: cmd) (Q: global_state -> Prop): Prop :=
+  forall (s1: global_state),
     P s1 ->
-    p > 0 ->
-    vPr s1 = p ->
     nPr s1 = 0 ->
     forall (s2: global_state),
       command_oaccess c (proj1_sig s1) (proj1_sig s2) ->
-      vPr s2 = p /\
+      same_covered_domain (rv_domain _ (proj1_sig s1)) (rv_domain _ (proj1_sig s2)) /\
       (nPr s2 = 0 -> Q s2).
 
-Definition TTriple {imp: Imperative} {sss: SmallStepSemantics} {psi: RandomDistribution ora} (P: global_state -> Prop) (c: cmd) (Q: global_state -> Prop): Prop :=
-  forall p (s1: global_state),
+Definition TTriple (P: global_state -> Prop) (c: cmd) (Q: global_state -> Prop): Prop :=
+  forall (s1: global_state),
     P s1 ->
-    p > 0 ->
-    vPr s1 = p ->
     nPr s1 = 0 ->
     forall (s2: global_state),
       command_oaccess c (proj1_sig s1) (proj1_sig s2) ->
-      vPr s2 = p /\
+      same_covered_domain (rv_domain _ (proj1_sig s1)) (rv_domain _ (proj1_sig s2)) /\
       nPr s2 = 0 /\
       Q s2.
-
-Definition Pr {imp: Imperative} {sss: SmallStepSemantics} {psi: RandomDistribution ora} (P: state -> Prop): global_state -> R :=
-  fun sigma => GProb (tm_set P sigma) / vPr sigma.
-
-Definition ConditionalPred {imp: Imperative} {sss: SmallStepSemantics} {psi: RandomDistribution ora} (P: global_state -> Prop) (condition: state -> Prop): global_state -> Prop :=
-  fun sigma => GProb (tm_set condition sigma) = 0 \/ exists sigma', is_substate (tm_meta_pred condition) sigma sigma' /\ P sigma'.
-
-
-Definition ProbEquiv {imp: Imperative} {sss: SmallStepSemantics} {psi: RandomDistribution ora} (sigma1 sigma2: global_state): Prop :=
-  forall P: MetaState state -> Prop,
-    GProb (valid_set P sigma1) = GProb (valid_set P sigma2).
 
 Require Import Morphisms.
